examples/ghc/lib/OccName.v
@@ -70,6 +70,11 @@ Require Import Module.
 Instance Uniquable_OccName : Unique.Uniquable OccName := {}.
 Admitted.
 
+(* Default values *)
+Import Panic.
+Instance Default_NameSpace : Default NameSpace := Build_Default _ VarName.
+Instance Default_OccName : Default OccName := Build_Default _ (Mk_OccName default default).
+
 (* Converted value declarations: *)
 
 (* Skipping instance Ord__OccName *)
