examples/ghc/lib/Var.v
@@ -19,7 +19,9 @@ Axiom error : forall {a:Type}, a.
 Require GHC.Base.
 Require GHC.Num.
 Require Name.
+Require Panic.
 Require Unique.
+Require Util.
 Import GHC.Base.Notations.
 
 (* Converted type declarations: *)
@@ -137,6 +139,11 @@ Definition varType (arg_6__ : Var) :=
 Instance Unique_Var : Unique.Uniquable Var.Var := {}.
 Admitted.
 
+Require Import Panic.
+Instance Default_IdScope : Default IdScope := Build_Default _ GlobalId.
+Instance Default_Var : Default Var := Build_Default _ (Mk_Id default default default default default default).
+
+
 (* Converted value declarations: *)
 
 (* The Haskell code containes partial or untranslateable code, which needs the
@@ -184,75 +191,15 @@ Local Definition Ord__Var_max : Var -> Var -> Var :=
 (* Translating `instance Data.Data.Data Var.Var' failed: OOPS! Cannot find
    information for class Qualified "Data.Data" "Data" unsupported *)
 
-Axiom globaliseId : forall {A : Type}, A.
-
-(* Translating `globaliseId' failed: using a record pattern for the unknown
-   constructor `Mk_TyVar' unsupported *)
-
-Axiom lazySetIdInfo : forall {A : Type}, A.
-
-(* Translating `lazySetIdInfo' failed: using a record pattern for the unknown
-   constructor `Mk_TyVar' unsupported *)
-
-Axiom setIdDetails : forall {A : Type}, A.
-
-(* Translating `setIdDetails' failed: using a record pattern for the unknown
-   constructor `Mk_TyVar' unsupported *)
-
-Axiom setIdExported : forall {A : Type}, A.
-
-(* Translating `setIdExported' failed: using a record pattern for the unknown
-   constructor `Mk_TyVar' unsupported *)
-
-Axiom setIdNotExported : forall {A : Type}, A.
-
-(* Translating `setIdNotExported' failed: using a record pattern for the unknown
-   constructor `Mk_TyVar' unsupported *)
-
-Axiom setTcTyVarDetails : forall {A : Type}, A.
-
-(* Translating `setTcTyVarDetails' failed: using a record pattern for the
-   unknown constructor `Mk_TyVar' unsupported *)
-
-Axiom setTyVarKind : forall {A : Type}, A.
-
-(* Translating `setTyVarKind' failed: using a record pattern for the unknown
-   constructor `Mk_TyVar' unsupported *)
-
-Axiom setVarName : forall {A : Type}, A.
-
-(* Translating `setVarName' failed: using a record pattern for the unknown
-   constructor `Mk_TyVar' unsupported *)
-
-Axiom setVarType : forall {A : Type}, A.
-
-(* Translating `setVarType' failed: using a record pattern for the unknown
-   constructor `Mk_TyVar' unsupported *)
-
-Axiom setVarUnique : forall {A : Type}, A.
-
-(* Translating `setVarUnique' failed: using a record pattern for the unknown
-   constructor `Mk_TyVar' unsupported *)
-
-Axiom updateTyVarKind : forall {A : Type}, A.
-
-(* Translating `updateTyVarKind' failed: using a record pattern for the unknown
-   constructor `Mk_TyVar' unsupported *)
-
-Axiom updateTyVarKindM : forall {A : Type}, A.
-
-(* Translating `updateTyVarKindM' failed: using a record pattern for the unknown
-   constructor `Mk_TyVar' unsupported *)
-
-Axiom updateVarType : forall {A : Type}, A.
-
-(* Translating `updateVarType' failed: using a record pattern for the unknown
-   constructor `Mk_TyVar' unsupported *)
-
-Axiom updateVarTypeM : forall {A : Type}, A.
-
-(* Translating `updateVarTypeM' failed: using a record pattern for the unknown
-   constructor `Mk_TyVar' unsupported *)
+Definition globaliseId : Id -> Id :=
+  fun id =>
+    match id with
+      | Mk_TyVar _ _ _ => error (GHC.Base.hs_string__ "Partial record update")
+      | TcTyVar _ _ _ _ => error (GHC.Base.hs_string__ "Partial record update")
+      | Mk_Id varName_46__ realUnique_47__ varType_48__ idScope_49__ id_details_50__
+              id_info_51__ => Mk_Id varName_46__ realUnique_47__ varType_48__ GlobalId
+                                    id_details_50__ id_info_51__
+    end.
 
 Definition isExportedId : Var -> bool :=
   fun arg_7__ =>
@@ -289,6 +236,19 @@ Definition isLocalId : Var -> bool :=
       | _ => false
     end.
 
+Definition setIdNotExported : Id -> Id :=
+  fun id =>
+    if andb Util.debugIsOn (negb (isLocalId id)) : bool
+    then (Panic.assertPanic (GHC.Base.hs_string__ "ghc/compiler/basicTypes/Var.hs")
+         (GHC.Num.fromInteger 431))
+    else match id with
+           | Mk_TyVar _ _ _ => error (GHC.Base.hs_string__ "Partial record update")
+           | TcTyVar _ _ _ _ => error (GHC.Base.hs_string__ "Partial record update")
+           | Mk_Id varName_21__ realUnique_22__ varType_23__ idScope_24__ id_details_25__
+                   id_info_26__ => Mk_Id varName_21__ realUnique_22__ varType_23__ (LocalId
+                                         NotExported) id_details_25__ id_info_26__
+         end.
+
 Definition isTKVar : Var -> bool :=
   fun arg_19__ =>
     match arg_19__ with
@@ -302,6 +262,16 @@ Definition isTyVar : Var -> bool :=
 
 Definition isTcTyVar : Var -> bool :=
   fun arg_17__ => match arg_17__ with | TcTyVar _ _ _ _ => true | _ => false end.
+
+Definition lazySetIdInfo : Id -> unit -> Var :=
+  fun id info =>
+    match id with
+      | Mk_TyVar _ _ _ => error (GHC.Base.hs_string__ "Partial record update")
+      | TcTyVar _ _ _ _ => error (GHC.Base.hs_string__ "Partial record update")
+      | Mk_Id varName_68__ realUnique_69__ varType_70__ idScope_71__ id_details_72__
+              id_info_73__ => Mk_Id varName_68__ realUnique_69__ varType_70__ idScope_71__
+                                    id_details_72__ info
+    end.
 
 Definition mkTcTyVar : Name.Name -> unit -> unit -> TyVar :=
   fun name kind details =>
@@ -324,8 +294,101 @@ Definition mkGlobalVar : unit -> Name.Name -> unit -> unit -> Id :=
 Definition mkExportedLocalVar : unit -> Name.Name -> unit -> unit -> Id :=
   fun details name ty info => mk_id name ty (LocalId Exported) details info.
 
+Definition setIdDetails : Id -> unit -> Id :=
+  fun id details =>
+    match id with
+      | Mk_TyVar _ _ _ => error (GHC.Base.hs_string__ "Partial record update")
+      | TcTyVar _ _ _ _ => error (GHC.Base.hs_string__ "Partial record update")
+      | Mk_Id varName_57__ realUnique_58__ varType_59__ idScope_60__ id_details_61__
+              id_info_62__ => Mk_Id varName_57__ realUnique_58__ varType_59__ idScope_60__
+                                    details id_info_62__
+    end.
+
+Definition setIdExported : Id -> Id :=
+  fun arg_32__ =>
+    match arg_32__ with
+      | (Mk_Id _ _ _ (LocalId _) _ _ as id) => match id with
+                                                 | Mk_TyVar _ _ _ => error (GHC.Base.hs_string__
+                                                                           "Partial record update")
+                                                 | TcTyVar _ _ _ _ => error (GHC.Base.hs_string__
+                                                                            "Partial record update")
+                                                 | Mk_Id varName_33__ realUnique_34__ varType_35__ idScope_36__
+                                                         id_details_37__ id_info_38__ => Mk_Id varName_33__
+                                                                                               realUnique_34__
+                                                                                               varType_35__ (LocalId
+                                                                                               Exported) id_details_37__
+                                                                                               id_info_38__
+                                               end
+      | (Mk_Id _ _ _ GlobalId _ _ as id) => id
+      | tv => Panic.panicStr (GHC.Base.hs_string__ "setIdExported") (Panic.noString
+                                                                    tv)
+    end.
+
+Definition setTcTyVarDetails : TyVar -> unit -> TyVar :=
+  fun tv details =>
+    match tv with
+      | Mk_TyVar _ _ _ => error (GHC.Base.hs_string__ "Partial record update")
+      | TcTyVar varName_83__ realUnique_84__ varType_85__ tc_tv_details_86__ =>
+        TcTyVar varName_83__ realUnique_84__ varType_85__ details
+      | Mk_Id _ _ _ _ _ _ => error (GHC.Base.hs_string__ "Partial record update")
+    end.
+
+Definition setTyVarKind : TyVar -> unit -> TyVar :=
+  fun tv k =>
+    match tv with
+      | Mk_TyVar varName_94__ realUnique_95__ varType_96__ => Mk_TyVar varName_94__
+                                                                       realUnique_95__ k
+      | TcTyVar varName_97__ realUnique_98__ varType_99__ tc_tv_details_100__ =>
+        TcTyVar varName_97__ realUnique_98__ k tc_tv_details_100__
+      | Mk_Id varName_101__ realUnique_102__ varType_103__ idScope_104__
+              id_details_105__ id_info_106__ => Mk_Id varName_101__ realUnique_102__ k
+                                                      idScope_104__ id_details_105__ id_info_106__
+    end.
+
+Definition setVarName : Var -> Name.Name -> Var :=
+  fun var new_name =>
+    match var with
+      | Mk_TyVar varName_202__ realUnique_203__ varType_204__ => Mk_TyVar new_name
+                                                                          (Unique.getKey (Unique.getUnique new_name))
+                                                                          varType_204__
+      | TcTyVar varName_205__ realUnique_206__ varType_207__ tc_tv_details_208__ =>
+        TcTyVar new_name (Unique.getKey (Unique.getUnique new_name)) varType_207__
+                tc_tv_details_208__
+      | Mk_Id varName_209__ realUnique_210__ varType_211__ idScope_212__
+              id_details_213__ id_info_214__ => Mk_Id new_name (Unique.getKey
+                                                      (Unique.getUnique new_name)) varType_211__ idScope_212__
+                                                      id_details_213__ id_info_214__
+    end.
+
 Definition setTyVarName : TyVar -> Name.Name -> TyVar :=
   setVarName.
+
+Definition setVarType : Id -> unit -> Id :=
+  fun id ty =>
+    match id with
+      | Mk_TyVar varName_184__ realUnique_185__ varType_186__ => Mk_TyVar
+                                                                 varName_184__ realUnique_185__ ty
+      | TcTyVar varName_187__ realUnique_188__ varType_189__ tc_tv_details_190__ =>
+        TcTyVar varName_187__ realUnique_188__ ty tc_tv_details_190__
+      | Mk_Id varName_191__ realUnique_192__ varType_193__ idScope_194__
+              id_details_195__ id_info_196__ => Mk_Id varName_191__ realUnique_192__ ty
+                                                      idScope_194__ id_details_195__ id_info_196__
+    end.
+
+Definition setVarUnique : Var -> Unique.Unique -> Var :=
+  fun var uniq =>
+    match var with
+      | Mk_TyVar varName_220__ realUnique_221__ varType_222__ => Mk_TyVar
+                                                                 (Name.setNameUnique (varName var) uniq) (Unique.getKey
+                                                                 uniq) varType_222__
+      | TcTyVar varName_223__ realUnique_224__ varType_225__ tc_tv_details_226__ =>
+        TcTyVar (Name.setNameUnique (varName var) uniq) (Unique.getKey uniq)
+                varType_225__ tc_tv_details_226__
+      | Mk_Id varName_227__ realUnique_228__ varType_229__ idScope_230__
+              id_details_231__ id_info_232__ => Mk_Id (Name.setNameUnique (varName var) uniq)
+                                                      (Unique.getKey uniq) varType_229__ idScope_230__ id_details_231__
+                                                      id_info_232__
+    end.
 
 Definition setTyVarUnique : TyVar -> Unique.Unique -> TyVar :=
   setVarUnique.
@@ -333,8 +396,61 @@ Definition setTyVarUnique : TyVar -> Unique.Unique -> TyVar :=
 Definition tyVarKind : TyVar -> unit :=
   varType.
 
+Definition updateTyVarKind : (unit -> unit) -> TyVar -> TyVar :=
+  fun update tv =>
+    match tv with
+      | Mk_TyVar varName_112__ realUnique_113__ varType_114__ => Mk_TyVar
+                                                                 varName_112__ realUnique_113__ (update (tyVarKind tv))
+      | TcTyVar varName_115__ realUnique_116__ varType_117__ tc_tv_details_118__ =>
+        TcTyVar varName_115__ realUnique_116__ (update (tyVarKind tv))
+                tc_tv_details_118__
+      | Mk_Id varName_119__ realUnique_120__ varType_121__ idScope_122__
+              id_details_123__ id_info_124__ => Mk_Id varName_119__ realUnique_120__ (update
+                                                      (tyVarKind tv)) idScope_122__ id_details_123__ id_info_124__
+    end.
+
+Definition updateTyVarKindM {m} `{(GHC.Base.Monad m)} : (unit -> m
+                                                        unit) -> TyVar -> m TyVar :=
+  fun update tv =>
+    update (tyVarKind tv) GHC.Base.>>= (fun k' =>
+      GHC.Base.return_ GHC.Base.$ (match tv with
+        | Mk_TyVar varName_130__ realUnique_131__ varType_132__ => Mk_TyVar
+                                                                   varName_130__ realUnique_131__ k'
+        | TcTyVar varName_133__ realUnique_134__ varType_135__ tc_tv_details_136__ =>
+          TcTyVar varName_133__ realUnique_134__ k' tc_tv_details_136__
+        | Mk_Id varName_137__ realUnique_138__ varType_139__ idScope_140__
+                id_details_141__ id_info_142__ => Mk_Id varName_137__ realUnique_138__ k'
+                                                        idScope_140__ id_details_141__ id_info_142__
+      end)).
+
 Definition tyVarName : TyVar -> Name.Name :=
   varName.
+
+Definition updateVarType : (unit -> unit) -> Id -> Id :=
+  fun f id =>
+    match id with
+      | Mk_TyVar varName_166__ realUnique_167__ varType_168__ => Mk_TyVar
+                                                                 varName_166__ realUnique_167__ (f (varType id))
+      | TcTyVar varName_169__ realUnique_170__ varType_171__ tc_tv_details_172__ =>
+        TcTyVar varName_169__ realUnique_170__ (f (varType id)) tc_tv_details_172__
+      | Mk_Id varName_173__ realUnique_174__ varType_175__ idScope_176__
+              id_details_177__ id_info_178__ => Mk_Id varName_173__ realUnique_174__ (f
+                                                      (varType id)) idScope_176__ id_details_177__ id_info_178__
+    end.
+
+Definition updateVarTypeM {m} `{GHC.Base.Monad m} : (unit -> m unit) -> Id -> m
+                                                    Id :=
+  fun f id =>
+    f (varType id) GHC.Base.>>= (fun ty' =>
+      GHC.Base.return_ (match id with
+                         | Mk_TyVar varName_148__ realUnique_149__ varType_150__ => Mk_TyVar
+                                                                                    varName_148__ realUnique_149__ ty'
+                         | TcTyVar varName_151__ realUnique_152__ varType_153__ tc_tv_details_154__ =>
+                           TcTyVar varName_151__ realUnique_152__ ty' tc_tv_details_154__
+                         | Mk_Id varName_155__ realUnique_156__ varType_157__ idScope_158__
+                                 id_details_159__ id_info_160__ => Mk_Id varName_155__ realUnique_156__ ty'
+                                                                         idScope_158__ id_details_159__ id_info_160__
+                       end)).
 
 Definition varUnique : Var -> Unique.Unique :=
   fun var => Unique.mkUniqueGrimily (realUnique var).
@@ -355,8 +471,10 @@ Program Instance Ord__Var : GHC.Base.Ord Var := fun _ k =>
       GHC.Base.min__ := Ord__Var_min |}.
 
 (* Unbound variables:
-     bool comparison error false negb true unit GHC.Base.Eq_ GHC.Base.Ord
-     GHC.Base.op_zeze__ GHC.Base.op_zg__ GHC.Base.op_zgze__ GHC.Base.op_zl__
-     GHC.Base.op_zlze__ GHC.Num.Int Name.Name Unique.Unique Unique.mkUniqueGrimily
-     Unique.nonDetCmpUnique
+     andb bool comparison error false negb true unit GHC.Base.Eq_ GHC.Base.Monad
+     GHC.Base.Ord GHC.Base.op_zd__ GHC.Base.op_zeze__ GHC.Base.op_zg__
+     GHC.Base.op_zgze__ GHC.Base.op_zgzgze__ GHC.Base.op_zl__ GHC.Base.op_zlze__
+     GHC.Base.return_ GHC.Num.Int Name.Name Name.setNameUnique Panic.assertPanic
+     Panic.noString Panic.panicStr Unique.Unique Unique.getKey Unique.getUnique
+     Unique.mkUniqueGrimily Unique.nonDetCmpUnique Util.debugIsOn
 *)
