examples/ghc/module-edits/Name/midamble.v
@@ -4,6 +4,9 @@ Import Module.
 
 (* Default values *)
 Import Panic.
+Instance Default_NameSort : Default NameSort := Build_Default _ System.
+Instance Default_Name : Default Name := Build_Default _ (Mk_Name default default default default).
+
 
 Instance Unique_Name : Unique.Uniquable Name.Name := {}.
 Admitted.
