examples/ghc/module-edits/OccName/midamble.v
@@ -3,3 +3,8 @@ Require Import Module.
 
 Instance Uniquable_OccName : Unique.Uniquable OccName := {}.
 Admitted.
+
+(* Default values *)
+Import Panic.
+Instance Default_NameSpace : Default NameSpace := Build_Default _ VarName.
+Instance Default_OccName : Default OccName := Build_Default _ (Mk_OccName default default).
