examples/ghc/module-edits/SrcLoc/midamble.v
@@ -1,0 +1,3 @@
+(* Default values *)
+Import Panic.
+Instance Default_SrcSpan : Default SrcSpan := Build_Default _ (UnhelpfulSpan default).
